Almost verified insertion

AVL.fst
@@ -15,7 +15,7 @@ let rec in_tree x = function
   | Leaf -> false
   | Node y l r _ -> y = x || in_tree x l || in_tree x r
 
-val all_more_than : k:int -> t:tree -> Tot bool
+val all_more_than : k:int -> t:tree -> Tot (r:bool {r <==> (forall x. in_tree x t ==> x > k)})
 let rec all_more_than k = function
 | Leaf -> true
 | Node y l r _ -> y > k && all_more_than k l && all_more_than k r
@@ -56,7 +56,7 @@ let rec has_real_heights = function
   | Leaf -> true
   | Node _ l r ah -> is_real_h ah l r && has_real_heights l && has_real_heights r
 
-val get_height : t:tree {has_real_heights t} -> Tot int
+val get_height : t:tree {has_real_heights t} -> Tot (r:int {r = real_height t})
 let get_height = function
     |Leaf -> 0
     | Node _ _ _ h -> h
@@ -79,7 +79,7 @@ type avl = t:tree {is_avl t}
 (* trees of height N *)
 type avln (n:int) = t:avl {real_height t = n}
 (* trees of height equal to that of another T *)
-type avlt (t:tree) = t':avln (real_height t)
+type avlt (t:tree) = avln (real_height t)
 type avll (k:int) = t:avl {all_less_than k t}
 (* trees of height equal to that of another T *)
 type avlr (k:int) = t:avl {all_more_than k t}
@@ -90,7 +90,7 @@ let empty = Leaf
 val singleton : int -> avln 1
 let singleton x =  Node x empty empty 1
 
-val mk_node : v:int -> l:(avll v) -> r:avlr v {has_bal 1 l r} -> Tot (avln (node_height l r ))
+val mk_node : v:int -> l:(avll v) -> r:avlr v {has_bal 1 l r} -> Tot (t:avln (node_height l r ) {(forall y. in_tree y t <==> in_tree y l \/ in_tree y r \/ v = y)})
 let mk_node v l r =
  let hl = get_height l in
  let hr = get_height r in
@@ -117,20 +117,10 @@ let right (Node _ _ r _) = r
 val left_of_avl_is_avll : t:avl{not_empty t} -> y:int {y == head t } -> Lemma(all_less_than y (left t))
 let left_of_avl_is_avll t y = ()
 
-(*
-val insert : x:int -> t:avl -> Tot avl
-let rec insert x = function
-  | Leaf -> singleton x
-  | Node y l r h ->
-    if x < y
-    then begin
-      left_of_avl_is_avll (Node y l r h) y;
-      mk_node y (insert x l) r
-    end
-    else mk_node y l (insert x r)
-*)
+val real_diff : s:tree -> t:tree -> Tot int
+let real_diff s t = real_height s - real_height t
 
-val diff : s:tree {has_real_heights s} -> t:tree {has_real_heights t} -> Tot (r:int {get_height s <= get_height t + r } )
+val diff : s:tree {has_real_heights s} -> t:tree {has_real_heights t} -> Tot (r:int {r = real_diff s t} )
 let diff s t = get_height s - get_height t
 
 val get_balfac : t:tree {has_real_heights t} -> Tot int
@@ -165,7 +155,7 @@ let all_more_intro v x l r  = ()
 val all_less_intro: v:int -> x:int {x < v} -> l:avll x {all_less_than v l} -> r:avlr x {all_less_than v r && has_bal 1 l r} -> Lemma ((all_less_than v (mk_node x l r)))
 let all_less_intro v x l r  = ()
 
-val balL0 : x:int -> l:avll x {is_not_heavy l} -> r:avlr x {is_left_big l r} -> avln (real_height l + 1)
+val balL0 : x:int -> l:avll x {is_not_heavy l} -> r:avlr x {is_left_big l r} -> Tot (t:avln (real_height l + 1) {(forall y. in_tree y t <==> in_tree y l \/ in_tree y r \/ x = y)})
 let balL0 x l r = match l with
   | (Node lv ll lr _) ->
     let y = mk_node x lr r in
@@ -173,12 +163,12 @@ let balL0 x l r = match l with
     mk_node lv ll y
   | _ -> admit ()
 
-val balLL : x:int -> l:avll x {is_left_heavy l} -> r:avlr x {is_left_big l r} -> avlt l
+val balLL : x:int -> l:avll x {is_left_heavy l} -> r:avlr x {is_left_big l r} -> Tot (avlt l)
 let balLL v (Node lv ll lr _) r =
   all_more_transitive lv v r;
   mk_node lv ll (mk_node v lr r)
 
-val eq_or_up : s:tree{has_real_heights s} -> t:tree{has_real_heights t} -> Tot (r:bool {r <==> diff t s = 0 \/ diff t s = 1})
+val eq_or_up : s:tree{has_real_heights s} -> t:tree{has_real_heights t} -> Tot bool
 let eq_or_up s t =
   let d = diff t s in
   d = 0 || d = 1
@@ -197,7 +187,7 @@ let big_ht l r t =
 val re_bal : l:tree {has_real_heights l} -> r:tree {has_real_heights r} -> t:tree{has_real_heights t} -> Tot bool
 let re_bal l r t = big_ht l r t && bal_ht l r t
 
-val balLR :x:int  -> l:avll x {is_right_heavy l} -> r:avlr x {is_left_big l r} -> Tot (avlt l)
+val balLR :x:int  -> l:avll x {is_right_heavy l} -> r:avlr x {is_left_big l r} -> Tot (t:avlt l  {(forall y. in_tree y t <==> in_tree y l \/ in_tree y r \/ x = y)})
 let balLR v l r = match l with
   | (Node lv ll (Node lrv lrl lrr lrh) lh) ->
     let y = mk_node v lrr r in
@@ -211,7 +201,7 @@ let balLR v l r = match l with
     admit()
 
 
-val balR0 : x:int  -> r:avlr x {is_not_heavy r} -> l:avll x {is_right_big l r} -> Tot (avln (real_height r + 1))
+val balR0 : x:int  -> r:avlr x {is_not_heavy r} -> l:avll x {is_right_big l r} -> Tot (t:avln (real_height r + 1) {(forall y. in_tree y t <==> in_tree y l \/ in_tree y r \/ x = y)})
 let balR0 x r l = match r with
   | (Node rv rl rr _) ->
     all_less_transitive rv x l;
@@ -221,12 +211,12 @@ let balR0 x r l = match r with
     admit ()
 
 
-val balRR : x:int -> l:avll x -> r:avlr x {is_right_big l r && is_right_heavy r} -> Tot (avlt r)
+val balRR : x:int -> l:avll x -> r:avlr x {is_right_big l r && is_right_heavy r} -> Tot (t:avlt r { (forall y. in_tree y t <==> in_tree y l \/ in_tree y r \/ x = y)})
 let balRR x l (Node rv rl rr _) =
   all_less_transitive rv x l;
   mk_node rv (mk_node x l rl) rr
 
-val balRL : x:int -> l: avll x -> r:avlr x {is_right_big l r && is_left_heavy r} -> Tot (avlt r)
+val balRL : x:int -> l: avll x -> r:avlr x {is_right_big l r && is_left_heavy r} -> Tot (t:avlt r {(forall y. in_tree y t <==> in_tree y l \/ in_tree y r \/ x = y)})
 let balRL x l = function
   | (Node rv (Node rlv rll rlr _) rr _) ->
     all_less_transitive rlv x l;
@@ -236,10 +226,11 @@ let balRL x l = function
     (* should be impossible *)
     admit ()
 
+val no_balancing_needed : l:tree {has_real_heights l } -> r:tree {has_real_heights r /\ has_bal 2 l r /\ not (is_left_big l r) /\ not (is_right_big l r)} -> Lemma (has_bal 1 l r)
+let no_balancing_needed l r = ()
 
-val bal : x:int -> l:avll x -> r:avlr x {has_bal 2 l r} -> t:avl {re_bal l r t /\ (forall y. in_tree y t <==> in_tree y l \/ in_tree y r \/ x = y)}
+val bal : x:int -> l:avll x -> r:avlr x {has_bal 2 l r} -> Tot (t:avl {re_bal l r t /\ (forall y. in_tree y t <==> in_tree y l \/ in_tree y r \/ x = y)})
 let bal v l r  =
-  admit ();
   let ilb = is_left_big l r in
   let irb = is_right_big l r in
   if (ilb && is_left_heavy l) then balLL v l r
@@ -248,74 +239,26 @@ let bal v l r  =
   else if (irb && is_left_heavy r) then balRL v l r
   else if (irb && is_right_heavy r) then balRR v l r
   else if (irb) then balR0 v r l
-  else mk_node v l r
-
-val minimum : t:tree {not_empty t} -> Tot int
-let rec minimum (Node x l r _) =
-  let lv = if not_empty l then minimum l else x in
-  let lr = if not_empty r then minimum r else x in
-  min( min x lv) lr
-
-
-val maximum : t:tree {not_empty t} -> Tot int
-let rec maximum (Node x l r _) =
-  let lv = if not_empty l then maximum l else x in
-  let lr = if not_empty r then maximum r else x in
-  max ( max x lv) lr
-
-val maximum_all_less_lemma : t:tree{not_empty t} -> Lemma (all_less_than (maximum t + 1) t )
-let maximum_all_less_lemma t = admit ()
-
-val all_less_minimum_lemma : v:int -> t:tree{all_less_than v t} -> Lemma (not_empty t ==> maximum t < v)
-let all_less_minimum_lemma v t = admit ()
-
-val elems : t:tree -> Tot (Set.set int)
-let rec elems = function
-  | Leaf -> Set.empty
-  | Node x l r _ ->  Set.union (Set.singleton x) (Set.union (elems l)  (elems r))
-
-
-(*val add_elems_prop : x:int -> t:tree -> s:tree -> Tot logical  *)
-let add_elems_prop x t s = (forall y. (Set.mem y (elems s) ) <==> (y == x \/  (Set.mem y (elems t))))
-
-
-val elems_less_than_lemma : v:int -> t:tree {forall y. (Set.mem y (elems t) ==> y < v)} -> Lemma (all_less_than v t)
-let elems_less_than_lemma v t = admit ()
-
-val less_than_elems_lemma : v:int -> t:tree {all_less_than v t} -> Lemma (forall y. (Set.mem y (elems t) ==> y < v))
-let less_than_elems_lemma v t = admit ()
-
-
-let add_elems_in_tree x t s = (forall y. (in_tree y s ) ==> (y == x \/ (in_tree y t)))
+  else begin
+    no_balancing_needed l r;
+    mk_node v l r
+  end
 
 
 val in_tree_less_than_lemma : v:int -> t:tree {forall y. (in_tree y t ==> y < v)} -> Lemma (all_less_than v t)
-let in_tree_less_than_lemma v t = admit ()
+let in_tree_less_than_lemma v t = ()
 
 
 val in_tree_more_than_lemma : v:int -> t:tree {forall y. (in_tree y t ==> y > v)} -> Lemma (all_more_than v t)
-let in_tree_more_than_lemma v t = admit ()
+let in_tree_more_than_lemma v t = ()
 
 
 val less_than_in_tree_lemma : v:int -> t:tree {all_less_than v t} -> Lemma (forall y. (in_tree y t ==> y < v))
-let less_than_in_tree_lemma v t = admit ()
+let less_than_in_tree_lemma v t = ()
 
 
 val more_than_in_tree_lemma : v:int -> t:tree {all_more_than v t} -> Lemma (forall y. (in_tree y t ==> y > v))
-let more_than_in_tree_lemma v t = admit ()
-
-
-val insert_bst : x:int -> t:tree {is_bst t} -> Tot (r:tree {is_bst r /\ (forall y. in_tree y r <==> (in_tree y t \/ x = y))})
-let rec insert_bst x t =
-  match t with
-  | Leaf -> singleton x
-  | Node n t1 t2 _ -> if x = n then      t
-                    else if x < n then Node n (insert_bst x t1) t2 (node_height (insert_bst x t1) t2)
-                    else               begin
-                      more_than_in_tree_lemma n t2;
-                      in_tree_more_than_lemma n (insert_bst x t2);
-                      Node n t1 (insert_bst x t2) (node_height t1 (insert_bst x t2))
-                    end
+let more_than_in_tree_lemma v t = ()
 
 val bal_not_empty : x:int -> l:avll x -> r:avlr x {has_bal 2 l r} -> Lemma (not_empty (bal x l r))
 let bal_not_empty x l r = ()
@@ -326,6 +269,11 @@ let bal_height x l r = ()
 val bal_in_tree : x:int -> l:avll x -> r:avlr x {has_bal 2 l r} -> Lemma (forall y. in_tree y (bal x l r) <==> in_tree y l \/ in_tree y r \/ x = y)
 let bal_in_tree x l r = ()
 
+val intro_diff_0_or_1_c :t:tree -> s:tree {real_height t - real_height s >= 0 /\ real_height t - real_height s <= 1} -> Lemma (real_diff t s = 0 \/ real_diff t s = 1)
+let intro_diff_0_or_1_c t s = ()
+
+val magic_lemma_bal : t:tree -> s:tree -> Lemma (real_height t - real_height s >= 0 /\ real_height t - real_height s <= 1)
+let magic_lemma_bal  t s = admit ()
 
 val insert: x:int -> s:avl -> Tot (t:avl {not_empty t /\ eq_or_up s t /\ (forall y. (in_tree y t) <==> (in_tree y s \/ x = y))})
 let rec insert x s = match s with
@@ -338,33 +286,16 @@ let rec insert x s = match s with
       bal_not_empty v insl r;
       bal_height v insl r;
       bal_in_tree v insl r;
-      assert (is_avl (bal v insl r));
-      assert (eq_or_up l insl);
-      assert (real_height s <= real_height (bal v insl r));
-      assert (real_height (bal v insl r) <= real_height s + 1);
-      assert (real_height (bal v insl r) - real_height s <= 1);
-      assert (diff (bal v insl r) s = 0 \/ diff (bal v insl r) s = 1);
-      assert (eq_or_up s (bal v insl r));
-      assert ( (forall y. (in_tree y insl) <==> (in_tree y l \/ x = y)));
-      admit ()
-    end else if x > v then begin
-      admit ()
-    end else s
-
-
-(*
-val insert: x:int -> s:avl -> Tot (t:avl {not_empty t /\ eq_or_up s t /\ (minimum t = (if is_empty s then x else min x (minimum s))) /\ (maximum t = (if is_empty s then x else max x (maximum s)))}) (decreases s)
-let rec insert x t = match t with
-  | (Node v l r n) ->
-    if x < v then begin
-      let insl = insert x l in
-      all_less_minimum_lemma v l;
-      assert (maximum insl <= v - 1);
-      maximum_all_less_lemma insl;
-      all_less_transitive v (maximum insl + 1) insl;
+      intro_diff_0_or_1_c (bal v insl r) s;
       bal v insl r
     end else if x > v then begin
-      bal v l (insert x r)
-    end else t
-  | Leaf -> singleton x
-*)
+      let insr = insert x r in
+      more_than_in_tree_lemma v r;
+      in_tree_more_than_lemma v insr;
+      bal_not_empty v l insr;
+      bal_height v l insr;
+      bal_in_tree v l insr;
+      magic_lemma_bal (bal v l insr) s;
+      intro_diff_0_or_1_c (bal v l insr) s;
+      bal v l insr
+    end else s
